reals/fast/CRArith.v
@@ -142,7 +142,7 @@ Hint Rewrite <- CRinv_Qinv : toCRring.
 CR forms a ring for the ring tactic.
 *)
 Lemma CR_ring_theory : 
- @ring_theory (ms CR) (' 0%Q) (' 1%Q) (ucFun2 CRplus) CRmult
+ @ring_theory CR (' 0%Q) (' 1%Q) (ucFun2 CRplus) CRmult
  (fun (x y:CR) => (x + - y)) CRopp (@ms_eq CR).
 Proof.
 split.
@@ -189,7 +189,7 @@ rapply CRmult_wd.
 rapply uc_wd.
 Qed.
 
-Add Ring CR_ring : CR_ring_theory (morphism CR_Q_ring_morphism, setoid (@msp_Xsetoid _ _ _ (@msp CR)) CR_ring_eq_ext, constants [CRcst], preprocess [CRring_pre]).
+Add Ring CR_ring : CR_ring_theory (morphism CR_Q_ring_morphism, setoid (@st_isSetoid (@msp_is_setoid CR)) CR_ring_eq_ext, constants [CRcst], preprocess [CRring_pre]).
 
 (** Relationship between strict and nonstrict positivity *)
 Lemma CRpos_nonNeg : forall x, CRpos x -> CRnonNeg x.
@@ -197,7 +197,7 @@ intros x [c Hx].
 cut ('0 <= x)%CR.
  unfold CRle.
  intros H.
- setoid_replace (x - '0)%CR with x in H by ring.
+ setoid_replace (x - '0)%CR with x using relation (@ms_eq CR) in H by ring.
  assumption.
 apply CRle_trans with (' c)%CR; auto with *.
 rewrite CRle_Qle; auto with *.
@@ -208,7 +208,7 @@ intros x [c Hx].
 cut (x <= '0)%CR.
  unfold CRle.
  intros H.
- setoid_replace ('0 - x)%CR with (-x)%CR in H by ring.
+ setoid_replace ('0 - x)%CR with (-x)%CR using relation (@ms_eq CR) in H by ring.
  intros e.
  rewrite <- (Qopp_involutive e).
  rewrite <- (Qopp_involutive (approximate x e)).
